compiler/src/compiler/Pipeline.v
@@ -1,0 +1,1485 @@
+Require Export Coq.Lists.List.
+Require Import Coq.ZArith.ZArith.
+Export ListNotations.
+Require Export coqutil.Decidable.
+Require        compiler.ExprImp.
+Require Export compiler.FlattenExprDef.
+Require Export compiler.FlattenExpr.
+Require        compiler.FlatImp.
+Require Export riscv.Spec.Machine.
+Require Export riscv.Platform.Run.
+Require Export riscv.Platform.RiscvMachine.
+Require Export riscv.Platform.MetricLogging.
+Require Export riscv.Utility.Monads.
+Require Import riscv.Utility.runsToNonDet.
+Require Export riscv.Platform.MetricRiscvMachine.
+Require Import coqutil.Z.Lia.
+Require Import compiler.NameGen.
+Require Import compiler.StringNameGen.
+Require Export compiler.util.Common.
+Require Export coqutil.Decidable.
+Require Export riscv.Utility.Encode.
+Require Import riscv.Spec.Decode.
+Require Export riscv.Spec.Primitives.
+Require Export riscv.Spec.MetricPrimitives.
+Require Import compiler.GoFlatToRiscv.
+Require Import riscv.Utility.MkMachineWidth.
+Require Export riscv.Proofs.DecodeEncode.
+Require Export riscv.Proofs.EncodeBound.
+Require Import riscv.Utility.Utility.
+Require Export riscv.Platform.Memory.
+Require Export riscv.Utility.InstructionCoercions.
+Require Import compiler.SeparationLogic.
+Require Import coqutil.Tactics.Simp.
+Require Import compiler.FlattenExprSimulation.
+Require Import compiler.Spilling.
+Require Import compiler.RegRename.
+Require Import compiler.FlatToRiscvSimulation.
+Require Import compiler.Simulation.
+Require Import compiler.RiscvEventLoop.
+Require Coq.Init.Byte.
+Require Import bedrock2.MetricLogging.
+Require Import compiler.FlatToRiscvCommon.
+Require Import compiler.FlatToRiscvFunctions.
+Require Import compiler.DivisibleBy4.
+Require Export coqutil.Word.SimplWordExpr.
+Require Import compiler.ForeverSafe.
+Require Export compiler.MemoryLayout.
+Require Import FunctionalExtensionality.
+Require Import coqutil.Tactics.autoforward.
+Require Import compiler.FitsStack.
+Import Utility.
+
+Existing Instance riscv.Spec.Machine.DefaultRiscvState.
+
+Open Scope Z_scope.
+
+Section WithWordAndMem.
+  Context {width: Z} {word: word.word width} {mem: map.map word byte}.
+
+  (* bedrock2.ptsto_bytes.ptsto_bytes takes an n-tuple of bytes, whereas this one takes a list of bytes *)
+  Definition ptsto_bytes: word -> list byte -> mem -> Prop := array ptsto (word.of_Z 1).
+
+  Definition mem_available(start pastend: word) : mem -> Prop :=
+    ex1 (fun anybytes: list byte =>
+      emp (Z.of_nat (List.length anybytes) = word.unsigned (word.sub pastend start)) *
+      (ptsto_bytes start anybytes))%sep.
+End WithWordAndMem.
+
+Module Import Pipeline.
+
+  Class parameters := {
+    W :> Words;
+    mem :> map.map word byte;
+    Registers :> map.map Z word;
+    string_keyed_map :> forall T: Type, map.map string T; (* abstract T for better reusability *)
+    trace := list (mem * string * list word * (mem * list word));
+    ExtSpec := trace -> mem -> string -> list word -> (mem -> list word -> Prop) -> Prop;
+    ext_spec : ExtSpec;
+    compile_ext_call : string_keyed_map Z -> Z -> Z -> FlatImp.stmt Z -> list Instruction;
+    M: Type -> Type;
+    MM :> Monad M;
+    RVM :> RiscvProgram M word;
+    PRParams :> PrimitivesParams M MetricRiscvMachine;
+  }.
+
+  Instance FlatToRiscvDef_parameters{p: parameters}: FlatToRiscvDef.FlatToRiscvDef.parameters := {|
+    iset := if Utility.width =? 32 then RV32I else RV64I;
+    FlatToRiscvDef.FlatToRiscvDef.compile_ext_call := compile_ext_call;
+  |}.
+
+  Instance FlattenExpr_parameters{p: parameters}: FlattenExpr.parameters := {
+    FlattenExpr.W := _;
+    FlattenExpr.locals := _;
+    FlattenExpr.mem := mem;
+    FlattenExpr.ext_spec := ext_spec;
+    FlattenExpr.NGstate := N;
+  }.
+
+  Instance FlatToRiscv_params{p: parameters}: FlatToRiscvCommon.parameters := {|
+    FlatToRiscvCommon.ext_spec := ext_spec;
+  |}.
+
+  Class assumptions{p: parameters}: Prop := {
+    word_riscv_ok :> RiscvWordProperties.word.riscv_ok word;
+    string_keyed_map_ok :> forall T, map.ok (string_keyed_map T);
+    Registers_ok :> map.ok Registers;
+    PR :> MetricPrimitives PRParams;
+    FlatToRiscv_hyps :> FlatToRiscvCommon.assumptions;
+    ext_spec_ok :> Semantics.ext_spec.ok (FlattenExpr.mk_Semantics_params FlattenExpr_parameters);
+    compile_ext_call_correct: forall resvars extcall argvars,
+        compiles_FlatToRiscv_correctly
+          compile_ext_call (FlatImp.SInteract resvars extcall argvars);
+    compile_ext_call_length_ignores_positions: forall stackoffset posmap1 posmap2 c pos1 pos2,
+      List.length (compile_ext_call posmap1 pos1 stackoffset c) =
+      List.length (compile_ext_call posmap2 pos2 stackoffset c);
+  }.
+
+End Pipeline.
+
+Section SIM.
+  Context {Frame1 State1: Type}.
+  Context (exec1: State1 -> (State1 -> Prop) -> Prop).
+  Context {Frame2 State2: Type}.
+  Context (exec2: State2 -> (State2 -> Prop) -> Prop).
+  Context (states_related: Frame1 -> Frame2 -> State1 -> State2 -> Prop).
+
+  Definition simulation f1 f2 :=
+      forall (P1: State1 -> Prop) (P2: State2 -> Prop),
+      (* read line below as "P2 must be implied by exists s1', states_related f1 f2 s1' s2' /\ P1 s1'"
+         or as "if P1 says s1' is an acceptable final state, then P2 must accept all s2' related to s1'" *)
+      (forall s1' s2', states_related f1 f2 s1' s2' -> P1 s1' -> P2 s2') ->
+      forall s1 s2, states_related f1 f2 s1 s2 -> exec1 s1 P1 -> exec2 s2 P2.
+
+  (* Note: The above could be simplified like this, but then P2 cannot be weakened and we need
+     to carry around a separate hypothesis requiring weakening for language 2. *)
+  Definition simulation_without_weakening f1 f2 := forall (P1: State1 -> Prop) s1 s2,
+      states_related f1 f2 s1 s2 ->
+      exec1 s1 P1 ->
+      exec2 s2 (fun s2' => exists s1', states_related f1 f2 s1' s2' /\ P1 s1').
+
+  Lemma simulation_alt: forall f1 f2, simulation f1 f2 -> simulation_without_weakening f1 f2.
+  Proof. unfold simulation, simulation_without_weakening. eauto 10. Qed.
+
+  Lemma simulation_alt_verboseproof: forall f1 f2, simulation f1 f2 -> simulation_without_weakening f1 f2.
+  Proof.
+    unfold simulation, simulation_without_weakening.
+    intros *. intro Sim. intros. eapply Sim. 2,3: eassumption.
+    clear. intros. eauto.
+  Qed.
+
+  Lemma simulation_alt':
+    (forall (P2 P2': State2 -> Prop), (forall s2, P2 s2 -> P2' s2) -> forall s2, exec2 s2 P2 -> exec2 s2 P2') ->
+    forall f1 f2, simulation_without_weakening f1 f2 -> simulation f1 f2.
+  Proof.
+    unfold simulation_without_weakening, simulation.
+    intros W. intros *. intros Sim. intros.
+    eapply W. 2: {
+      eapply Sim. 1: eassumption. eassumption.
+    }
+    cbv beta.
+    intros s (s1' & ? & ?).
+    eauto.
+  Qed.
+
+End SIM.
+
+Section COMPOSE.
+  Context {Frame1 State1: Type}.
+  Context (exec1: State1 -> (State1 -> Prop) -> Prop).
+  Context {Frame2 State2: Type}.
+  Context (exec2: State2 -> (State2 -> Prop) -> Prop).
+  Context {Frame3 State3: Type}.
+  Context (exec3: State3 -> (State3 -> Prop) -> Prop).
+  Context (frelated12: Frame1 -> Frame2 -> Prop).
+  Context (frelated23: Frame2 -> Frame3 -> Prop).
+  Context (related12: Frame1 -> Frame2 -> State1 -> State2 -> Prop).
+  Context (related23: Frame2 -> Frame3 -> State2 -> State3 -> Prop).
+
+(*
+  Definition compose_frelated: Frame1 -> Frame3 -> Prop :=
+    fun f1 f3 => exists f2, frelated12 f1 f2 /\ frelated23 f2 f3.
+*)
+
+  Definition compose_related(f2: Frame2)(f1: Frame1)(f3: Frame3): State1 -> State3 -> Prop :=
+    fun s1 s3 => exists s2, related12 f1 f2 s1 s2 /\ related23 f2 f3 s2 s3.
+
+  Lemma compose_simulation
+        (S12: forall f1 f2, frelated12 f1 f2 -> simulation exec1 exec2 related12 f1 f2)
+        (S23: forall f2 f3, frelated23 f2 f3 -> simulation exec2 exec3 related23 f2 f3):
+    forall f1 f3 f2, frelated12 f1 f2 -> frelated23 f2 f3 ->
+    simulation exec1 exec3 (compose_related f2) f1 f3.
+  Proof.
+  Abort.
+(* how to say that middle frame is still the same in post? above can, but makes simulation uncomposable
+   previous approach didn't achieve that
+
+
+each simulation holds under some assumptions about frames, and assuming intermediate frames exist
+compose two simulations that live under assumptions, combining the list of assumptions?
+
+
+forall (a1: A1) ... (an: An), A
+forall (b1: B1) ... (bm: Bm), B
+
+forall (a1: A1) ... (an: An)(b1: B1) ... (bm: Bm), compose A B
+
+forall (a: {A1 * ... An | P}), A
+
+real parameterization only needed in last phase
+
+but previous phases might have target-language-state validity (and thus "related") depend on source program
+
+
+
+    unfold simulation, compose_frelated, compose_related in *.
+    intros f1 f3 (f2 & HF12 & HF23) P1 P3 P13 s1 s3 (f2 & s2 & HR12 & HR23) Ex1.
+    eapply S23. 2: exact HR23. 2: {
+      eapply S12 with (P2 := (fun s2' => exists s1', related12 f1 s1' f2 s2' /\ P1 s1')).
+      2: exact HR12. 2: exact Ex1. eauto. }
+    intros s2' s3' HR23' (s1' & HR12' & p1). eauto.
+  Qed.
+
+*)
+
+(* simulation  nil/cons ? *)
+
+End COMPOSE.
+
+Arguments compose_simulation {_} {_} {_} {_} {_} {_} {_} {_} {_} {_} {_}.
+
+Section Pipeline1.
+
+  Context {p: parameters}.
+  Context {h: assumptions}.
+
+  Add Ring wring : (word.ring_theory (word := word))
+      (preprocess [autorewrite with rew_word_morphism],
+       morphism (word.ring_morph (word := word)),
+       constants [word_cst]).
+
+  Instance mk_FlatImp_ext_spec_ok:
+    FlatImp.ext_spec.ok  string (FlattenExpr.mk_FlatImp_params FlattenExpr_parameters).
+  Proof.
+    destruct h. destruct ext_spec_ok0.
+    constructor.
+    all: intros; eauto.
+    eapply intersect; eassumption.
+  Qed.
+
+  Instance FlattenExpr_hyps: FlattenExpr.assumptions FlattenExpr_parameters.
+  Proof.
+    constructor.
+    - apply (string_keyed_map_ok (p := p) (@word (@FlattenExpr.W (@FlattenExpr_parameters p)))).
+    - exact mem_ok.
+    - apply (string_keyed_map_ok (p := p) (list string * list string * Syntax.cmd.cmd)).
+    - apply (string_keyed_map_ok (p := p) (list string * list string * FlatImp.stmt string)).
+    - apply mk_FlatImp_ext_spec_ok.
+  Qed.
+
+  Local Notation source_env := (@string_keyed_map p (list string * list string * Syntax.cmd)).
+  Local Notation flat_env := (@string_keyed_map p (list string * list string * FlatImp.stmt string)).
+  Local Notation renamed_env := (@string_keyed_map p (list Z * list Z * FlatImp.stmt Z)).
+
+  Definition flattenPhase(prog: source_env): option flat_env := flatten_functions prog.
+  Definition renamePhase(prog: flat_env): option renamed_env :=
+    rename_functions prog.
+  Definition spillingPhase(prog: renamed_env): option renamed_env := Some (spill_functions prog).
+
+  (* Note: we could also track code size from the source program all the way to the target
+     program, and a lot of infrastructure is already there, will do once/if we want to get
+     a total compiler.
+     Returns the fun_pos_env so that users know where to jump to call the compiled functions. *)
+  Definition riscvPhase(prog: renamed_env):
+    option (list Instruction * funname_env Z * Z) :=
+    bind_opt stack_words_needed <- stack_usage prog;
+    let positions := FlatToRiscvDef.build_fun_pos_env prog in
+    let '(i, _) := FlatToRiscvDef.compile_funs positions prog in
+    Some (i, positions, stack_words_needed).
+
+  Definition composePhases{A B C: Type}(phase1: A -> option B)(phase2: B -> option C)(a: A) :=
+    match phase1 a with
+    | Some b => phase2 b
+    | None => None
+    end.
+
+  Definition composed_compile: source_env -> option (list Instruction * funname_env Z * Z) :=
+    (composePhases flattenPhase
+    (composePhases renamePhase
+    (composePhases spillingPhase
+                   riscvPhase))).
+
+  Definition FlatState(varname: Type){pp : FlatImp.parameters varname}: Type :=
+    FlatImp.env * FlatImp.stmt varname * bool * FlatImp.trace * FlatImp.mem * FlatImp.locals * MetricLog.
+
+  Definition flatExec{varname: Type}{pp : FlatImp.parameters varname}:
+    FlatState varname -> (FlatState varname -> Prop) -> Prop :=
+    fun '(e, s, done, t, m, l, mc) post =>
+      done = false /\
+      FlatImp.exec e s t m l mc (fun t' m' l' mc' => post (e, s, true, t', m', l', mc')).
+
+  (* Note: contrary to GhostConsts, this record only contains risc-v-related types, no FlatImp-related types *)
+  Record RiscvFrame: Type := {
+    addr_functions: word;
+    insts_functions: list Instruction;
+    addr_snippet: word;
+    insts_snippet: list Instruction;
+    stack_start: word;
+    stack_pastend: word;
+    xframe: mem -> Prop;
+    dframe: mem -> Prop;
+  }.
+
+  Definition satisfiesRiscvFrame(done: bool)(f: RiscvFrame)(mach: MetricRiscvMachine): Prop :=
+      (program iset f.(addr_functions) f.(insts_functions) *
+       program iset f.(addr_snippet) f.(insts_snippet) *
+       mem_available f.(stack_start) f.(stack_pastend) *
+       f.(dframe) * f.(xframe)
+      )%sep mach.(getMem) /\
+      subset (footpr (program iset f.(addr_functions) f.(insts_functions) *
+                      program iset f.(addr_snippet) f.(insts_snippet) *
+                      f.(xframe))%sep)
+             (of_list (getXAddrs mach)) /\
+      word.unsigned (mach.(getPc)) mod 4 = 0 /\
+      mach.(getPc) = (if done
+                      then word.add f.(addr_snippet) (word.of_Z (4 * Z.of_nat (length f.(insts_snippet))))
+                      else f.(addr_snippet)) /\
+      mach.(getNextPc) = word.add mach.(getPc) (word.of_Z 4) /\
+      regs_initialized mach.(getRegs) /\
+      map.get mach.(getRegs) RegisterNames.sp = Some f.(stack_pastend) /\
+      (* configured by PrimitivesParams, can contain invariants needed for external calls *)
+      valid_machine mach.
+
+  Definition flat_related_to_riscv
+             (frame1: @FlatImp.env Z _ * FlatImp.stmt Z)(s1: FlatState Z)
+             (frame2: RiscvFrame)(s2: MetricRiscvMachine): Prop :=
+    let '(e, c, done, t, m, l, mc) := s1 in
+    frame1 = (e, c) /\
+    map.extends s2.(getRegs) l /\
+    s2.(getLog) = t /\
+    fits_stack 0 (word.unsigned (word.sub frame2.(stack_pastend) frame2.(stack_start))) e c /\
+    FlatToRiscvDef.stmt_not_too_big c /\
+    FlatToRiscvDef.valid_FlatImp_vars c /\
+    let relpos := (word.unsigned (word.sub frame2.(addr_snippet) frame2.(addr_functions))) in
+    let e_pos := FlatToRiscvDef.build_fun_pos_env e in
+    fst (FlatToRiscvDef.compile_funs e_pos e) = frame2.(insts_functions) /\
+    FlatToRiscvDef.compile_stmt e_pos relpos 0 c = frame2.(insts_snippet) /\
+    satisfiesRiscvFrame done frame2 s2 /\
+    good_e_impl e e_pos.
+
+  Axiom TODO: False.
+
+(*
+  Lemma flatToRiscvSim: simulation flatExec FlatToRiscvCommon.runsTo flat_related_to_riscv.
+  Proof.
+    unfold simulation, flatExec, FlatState, FlatImp.SimExec, flat_related_to_riscv.
+    intros.
+    destruct s1 as ((((((e & c) & done) & t) & m) & l) & mc).
+    destruct_RiscvMachine s2.
+    simp.
+    eapply runsTo_weaken.
+    - specialize compile_stmt_correct with (1 := @compile_ext_call_correct _ h).
+      unfold compiles_FlatToRiscv_correctly. intros compile_stmt_correct.
+      eapply compile_stmt_correct.  all: case TODO. with (g := f2); clear compile_stmt_correct; simpl.
+      + eassumption.
+      + clear. intros k v ?. eassumption.
+      + assumption.
+      + eauto using fits_stack_call.
+      + eassumption.
+      + eassumption.
+      + eassumption.
+      + assert (word.ok word) by exact Utility.word_ok.
+        solve_divisibleBy4.
+        case TODO.
+      + assert (word.ok word) by exact Utility.word_ok.
+        solve_divisibleBy4.
+        case TODO.
+      + (* TODO why are these manual steps needed? *)
+        case TODO.
+      + assert (word.ok word) by exact Utility.word_ok.
+        case TODO.
+      + assumption.
+    - simpl. intros. simp.
+      eapply H. 2: eassumption.
+      cbv beta iota.
+      repeat match goal with
+             | |- _ /\ _ => split
+             | _ => eassumption
+             | _ => reflexivity
+             end.
+
+      Unshelve. all: case TODO.
+    - case TODO.
+  Qed.
+*)
+
+  Definition spilling_related
+             (frame1: @FlatImp.env Z _ * FlatImp.stmt Z)(s1: FlatState Z)
+             (frame2: @FlatImp.env Z _ * FlatImp.stmt Z)(s2: FlatState Z) :=
+    let '(e1, c1, done1, t1, m1, l1, mc1) := s1 in
+    let '(e2, c2, done2, t2, m2, l2, mc2) := s2 in
+    frame1 = (e1, c1) /\
+    frame2 = (e2, c2) /\
+    done1 = done2 /\
+    c2 = spill_stmt c1 /\
+    exists maxvar (fpval: word),
+      Spilling.envs_related e1 e2 /\
+      Spilling.valid_vars_src maxvar c1 /\
+      Spilling.related ext_spec maxvar (emp True) fpval t1 m1 l1 t2 m2 l2.
+
+  Lemma spilling_sim: simulation flatExec flatExec spilling_related.
+  Proof.
+    unfold simulation, flatExec, spilling_related. intros f1 f2 P1 P2 R.
+    intros ((((((e1 & c1) & done1) & t1) & m1) & l1) & mc1) ((((((e2 & c2) & done2) & t2) & m2) & l2) & mc2).
+    intros. simp. split; [reflexivity|].
+    eapply FlatImp.exec.weaken.
+    - eapply spilling_correct; eassumption.
+    - cbv beta. intros. simp. eapply R. 2: eassumption. simpl.
+      eauto 10.
+  Qed.
+
+  Definition renaming_related
+             (frame1: @FlatImp.env string _ * FlatImp.stmt string)(s1: FlatState string)
+             (frame2: @FlatImp.env Z _ * FlatImp.stmt Z)(s2: FlatState Z) :=
+    let '(e1, c1, done1, t1, m1, l1, mc1) := s1 in
+    let '(e2, c2, done2, t2, m2, l2, mc2) := s2 in
+    frame1 = (e1, c1) /\
+    frame2 = (e2, c2) /\
+    done1 = done2 /\
+    RegRename.envs_related e1 e2 /\
+    (exists r' av', RegRename.rename map.empty c1 lowest_available_impvar = Some (r', c2, av')) /\
+    t1 = t2 /\
+    m1 = m2 /\
+    (done1 = false -> l1 = map.empty /\ l2 = map.empty /\ mc1 = mc2).
+
+  Lemma renaming_sim: simulation flatExec flatExec renaming_related.
+  Proof.
+    unfold simulation, flatExec, renaming_related. intros f1 f2 P1 P2 R.
+    intros ((((((e1 & c1) & done1) & t1) & m1) & l1) & mc1) ((((((e2 & c2) & done2) & t2) & m2) & l2) & mc2).
+    intros. simp. split; [reflexivity|]. specialize (Hp3 eq_refl). simp.
+    pose proof Hp1 as A.
+    apply rename_props in A;
+      [|eapply map.empty_injective|eapply dom_bound_empty].
+    simp.
+    eapply FlatImp.exec.weaken.
+    - eapply rename_correct.
+      1: eassumption.
+      1: eassumption.
+      3: {
+        eapply Ap2. eapply TestLemmas.extends_refl.
+      }
+      1: eassumption.
+      1: eassumption.
+      unfold states_compat. intros *. intro B.
+      erewrite map.get_empty in B. discriminate.
+    - simpl. intros. simp.
+      eapply R. 2: eassumption. simpl. clear R. intuition (discriminate || eauto).
+  Qed.
+
+  Definition SrcState: Type :=
+    Semantics.env * Syntax.cmd * bool * Semantics.trace * Semantics.mem * Semantics.locals * MetricLog.
+
+  Definition srcExec: SrcState -> (SrcState -> Prop) -> Prop :=
+    fun '(e, c, done, t, m, l, mc) post =>
+      done = false /\
+      Semantics.exec e c t m l mc (fun t' m' l' mc' => post (e, c, true, t', m', l', mc')).
+
+  Definition flattening_related
+             (frame1: Semantics.env * Syntax.cmd)(s1: SrcState)
+             (frame2: @FlatImp.env string _ * FlatImp.stmt string)(s2: FlatState string) :=
+    let '(e1, c1, done1, t1, m1, l1, mc1) := s1 in
+    let '(e2, c2, done2, t2, m2, l2, mc2) := s2 in
+    frame1 = (e1, c1) /\
+    frame2 = (e2, c2) /\
+    done1 = done2 /\
+    ExprImp2FlatImp c1 = c2 /\
+    flatten_functions e1 = Some e2 /\
+    t1 = t2 /\
+    m1 = m2 /\
+    (done1 = false -> l1 = map.empty /\ l2 = map.empty /\ mc1 = mc2).
+
+  Lemma flattening_sim: simulation srcExec flatExec flattening_related.
+  Proof.
+    unfold simulation, srcExec, flatExec, flattening_related, ExprImp2FlatImp. intros f1 f2 P1 P2 R.
+    intros ((((((e1 & c1) & done1) & t1) & m1) & l1) & mc1) ((((((e2 & c2) & done2) & t2) & m2) & l2) & mc2).
+    intros. simp. split; [reflexivity|]. specialize (Hp2 eq_refl). simp.
+    eapply FlatImp.exec.weaken.
+    - eapply @flattenStmt_correct_aux with (eH := e1).
+      + typeclasses eauto.
+      + eassumption.
+      + eassumption.
+      + reflexivity.
+      + match goal with
+        | |- ?p = _ => rewrite (surjective_pairing p)
+        end.
+        reflexivity.
+      + intros x k A. rewrite map.get_empty in A. discriminate.
+      + unfold map.undef_on, map.agree_on. intros. reflexivity.
+      + eapply freshNameGenState_disjoint.
+    - simpl. intros. simp. eapply R. 2: eassumption. simpl. intuition (discriminate || eauto).
+  Qed.
+
+  Definition related: Semantics.env * Syntax.cmd -> SrcState -> RiscvFrame -> MetricRiscvMachine -> Prop :=
+    (compose_related flattening_related
+    (compose_related renaming_related
+    (compose_related spilling_related
+                     flat_related_to_riscv))).
+
+  Lemma sim: simulation srcExec FlatToRiscvCommon.runsTo related.
+  Proof.
+    exact (compose_simulation flattening_sim
+          (compose_simulation renaming_sim
+          (compose_simulation spilling_sim
+                              flatToRiscvSim))).
+  Qed.
+
+  Lemma rename_fun_valid: forall argnames retnames body impl',
+      rename_fun (argnames, retnames, body) = Some impl' ->
+      NoDup argnames ->
+      NoDup retnames ->
+      FlatImp.stmt_size body < 2 ^ 10 ->
+      FlatToRiscvDef.valid_FlatImp_fun impl'.
+  Proof.
+    unfold rename_fun, FlatToRiscvDef.valid_FlatImp_fun.
+    intros.
+    simp.
+    eapply rename_binds_props in E; cycle 1.
+    { eapply map.empty_injective. }
+    { eapply dom_bound_empty. }
+    simp.
+    eapply rename_binds_props in E0; cycle 1.
+    { assumption. }
+    { assumption. }
+    simp.
+    pose proof E1 as E1'.
+    eapply rename_props in E1; cycle 1.
+    { assumption. }
+    { assumption. }
+    simp.
+    set (lowest_nonregister := 32).
+    assert (Z.leb z1 lowest_nonregister = true) as E2 by case TODO.
+    ssplit.
+    - eapply Forall_impl. 2: {
+        eapply map.getmany_of_list_in_map. eassumption.
+      }
+      simpl.
+      intros. simp.
+      match goal with
+      | X: _ |- _ => specialize X with (1 := H); rename X into A
+      end.
+      destruct A as [A | A].
+      + apply Zle_bool_imp_le in E2.
+        unfold FlatToRiscvDef.valid_FlatImp_var, lowest_available_impvar, lowest_nonregister in *.
+        blia.
+      + rewrite map.get_empty in A. discriminate A.
+    - eapply Forall_impl. 2: {
+        eapply map.getmany_of_list_in_map. eassumption.
+      }
+      simpl.
+      intros. simp.
+      match goal with
+      | X: _ |- _ => specialize X with (1 := H); rename X into A
+      end.
+      destruct A as [A | A].
+      + apply Zle_bool_imp_le in E2.
+        unfold FlatToRiscvDef.valid_FlatImp_var, lowest_available_impvar, lowest_nonregister in *.
+        blia.
+      + match goal with
+        | X: _ |- _ => specialize X with (1 := A); rename X into B
+        end.
+        destruct B as [B | B].
+        * apply Zle_bool_imp_le in E2.
+          unfold FlatToRiscvDef.valid_FlatImp_var, lowest_available_impvar, lowest_nonregister in *.
+          blia.
+        * rewrite map.get_empty in B. discriminate B.
+    - eapply FlatImp.ForallVars_stmt_impl; [|eassumption].
+      simpl. intros. simp.
+      match goal with
+      | X: _ |- _ => specialize X with (1 := H); rename X into A
+      end.
+      destruct A as [A | A].
+      + apply Zle_bool_imp_le in E2.
+        unfold FlatToRiscvDef.valid_FlatImp_var, lowest_available_impvar, lowest_nonregister in *.
+        blia.
+      + match goal with
+        | X: _ |- _ => specialize X with (1 := A); rename X into B
+        end.
+        destruct B as [B | B].
+        * apply Zle_bool_imp_le in E2.
+          unfold FlatToRiscvDef.valid_FlatImp_var, lowest_available_impvar, lowest_nonregister in *.
+          blia.
+        * match goal with
+          | X: _ |- _ => specialize X with (1 := B); rename X into C
+          end.
+          destruct C as [C | C].
+          -- apply Zle_bool_imp_le in E2.
+             unfold FlatToRiscvDef.valid_FlatImp_var, lowest_available_impvar, lowest_nonregister in *.
+             blia.
+          -- rewrite map.get_empty in C. discriminate C.
+    - eapply map.getmany_of_list_injective_NoDup. 3: eassumption. all: eassumption.
+    - eapply map.getmany_of_list_injective_NoDup. 3: eassumption. all: eassumption.
+    - unfold FlatToRiscvDef.stmt_not_too_big.
+      pose proof (rename_preserves_stmt_size _ _ _ _ _ _ E1') as M.
+      rewrite <- M.
+      assumption.
+  Qed.
+
+  Local Instance map_ok': @map.ok (@word (@W p)) Init.Byte.byte (@mem p) := mem_ok.
+
+  Lemma get_build_fun_pos_env: forall e f,
+      map.get e f <> None ->
+      exists pos, map.get (FlatToRiscvDef.build_fun_pos_env e) f = Some pos.
+  Proof.
+    intros pos0 e.
+    unfold FlatToRiscvDef.build_fun_pos_env, FlatToRiscvDef.compile_funs.
+    eapply map.fold_spec.
+    - intros. rewrite map.get_empty in H. congruence.
+    - intros. destruct r as [ insts env]. simpl.
+      rewrite map.get_put_dec in H1.
+      rewrite map.get_put_dec.
+      destruct_one_match; eauto.
+  Qed.
+
+  Local Definition FlatImp__word_eq : FlatImp.word -> FlatImp.word -> bool := word.eqb.
+  Local Instance  EqDecider_FlatImp__word_eq : EqDecider FlatImp__word_eq.
+  Proof. eapply word.eqb_spec. Unshelve. exact word_ok. Qed.
+
+  Lemma mem_available_to_exists: forall start pastend m P,
+      (mem_available start pastend * P)%sep m ->
+      exists anybytes,
+        Z.of_nat (List.length anybytes) = word.unsigned (word.sub pastend start) /\
+        (ptsto_bytes start anybytes * P)%sep m.
+  Proof.
+    unfold mem_available. intros * H.
+    eapply sep_ex1_l in H. (* semicolon here fails *) destruct H.
+    eapply sep_assoc in H.
+    eapply sep_emp_l in H. destruct H.
+    eauto.
+  Qed.
+
+  Definition mem_to_available: forall start pastend m P anybytes,
+     Z.of_nat (List.length anybytes) = word.unsigned (word.sub pastend start) ->
+     (ptsto_bytes start anybytes * P)%sep m ->
+     (mem_available start pastend * P)%sep m.
+  Proof.
+    unfold mem_available. intros * H Hsep.
+    eapply sep_ex1_l. eexists. eapply sep_assoc. eapply sep_emp_l. eauto.
+  Qed.
+
+  Lemma get_compile_funs_pos: forall e,
+      let '(insts, posmap) := FlatToRiscvDef.compile_funs map.empty e in
+      forall f impl, map.get e f = Some impl -> exists pos2, map.get posmap f = Some pos2 /\ pos2 mod 4 = 0.
+  Proof.
+    intros e.
+    unfold FlatToRiscvDef.compile_funs.
+    eapply map.fold_spec.
+    - intros. rewrite map.get_empty in H. congruence.
+    - intros. destruct r as [ insts env]. simpl.
+      intros.
+      rewrite map.get_put_dec in H1.
+      rewrite map.get_put_dec.
+      destruct_one_match; eauto.
+      eexists. split; [reflexivity|].
+      solve_divisibleBy4.
+  Qed.
+
+  Lemma mod_2width_mod_bytes_per_word: forall x,
+      (x mod 2 ^ width) mod bytes_per_word = x mod bytes_per_word.
+  Proof.
+    intros.
+    rewrite <- Znumtheory.Zmod_div_mod.
+    - reflexivity.
+    - unfold bytes_per_word. destruct width_cases as [E | E]; rewrite E; reflexivity.
+    - destruct width_cases as [E | E]; rewrite E; reflexivity.
+    - unfold Z.divide.
+      exists (2 ^ width / bytes_per_word).
+      unfold bytes_per_word, Memory.bytes_per_word.
+      destruct width_cases as [E | E]; rewrite E; reflexivity.
+  Qed.
+
+  Lemma stack_length_divisible: forall (ml: MemoryLayout) {mlOk: MemoryLayoutOk ml},
+    word.unsigned (word.sub (MemoryLayout.stack_pastend ml) (MemoryLayout.stack_start ml)) mod bytes_per_word = 0.
+  Proof.
+    intros.
+    destruct mlOk.
+    rewrite word.unsigned_sub. unfold word.wrap.
+    rewrite mod_2width_mod_bytes_per_word.
+    rewrite Zminus_mod.
+    rewrite stack_start_aligned.
+    rewrite stack_pastend_aligned.
+    rewrite Z.sub_diag.
+    apply Zmod_0_l.
+  Qed.
+
+  Lemma program_mod_4_0: forall a instrs R m,
+      instrs <> [] ->
+      (program iset a instrs * R)%sep m ->
+      word.unsigned a mod 4 = 0.
+  Proof.
+    intros.
+    destruct instrs as [|instr instrs]. 1: congruence.
+    simpl in *.
+    unfold sep, ptsto_instr, sep, emp in *.
+    simp.
+    assumption.
+  Qed.
+
+  Lemma compile_funs_nonnil: forall e positions positions' f impl instrs,
+      map.get e f = Some impl ->
+      FlatToRiscvDef.compile_funs positions e = (instrs, positions') ->
+      instrs <> [].
+  Proof.
+    intros e positions.
+    unfold FlatToRiscvDef.compile_funs.
+    eapply map.fold_spec; intros.
+    - rewrite map.get_empty in H.
+      discriminate.
+    - rewrite map.get_put_dec in H1.
+      destr (k =? f)%string.
+      + subst.
+        unfold FlatToRiscvDef.add_compiled_function in H2. simp.
+        unfold FlatToRiscvDef.compile_function.
+        destruct impl as [ [args res] body ].
+        intro C. destruct l; discriminate.
+      + specialize H0 with (1 := H1).
+        destruct r as [ instrs'' positions'' ].
+        specialize H0 with (1 := eq_refl).
+        intro C. subst instrs.
+        unfold FlatToRiscvDef.add_compiled_function in H2. simp.
+        unfold FlatToRiscvDef.compile_function in *.
+        destruct v as [ [args res] body ].
+        destruct instrs''; discriminate.
+  Qed.
+
+  Ltac ignore_positions :=
+    repeat match goal with
+           | |- _ => reflexivity
+           | |- _ => rewrite !List.app_length
+           | |- _ => solve [eauto]
+           | |- _ => progress simpl
+           | |- S _ = S _ => f_equal
+           | |- (_ + _)%nat = (_ + _)%nat => f_equal
+           end.
+
+  Lemma compile_stmt_length_ignores_positions: forall posmap1 posmap2 c stackoffset pos1 pos2,
+      List.length (FlatToRiscvDef.compile_stmt posmap1 pos1 stackoffset c) =
+      List.length (FlatToRiscvDef.compile_stmt posmap2 pos2 stackoffset c).
+  Proof.
+    induction c; intros; ignore_positions.
+    apply compile_ext_call_length_ignores_positions.
+  Qed.
+
+  Lemma compile_function_length_ignores_positions: forall posmap1 posmap2 pos1 pos2 impl,
+      List.length (FlatToRiscvDef.compile_function posmap1 pos1 impl) =
+      List.length (FlatToRiscvDef.compile_function posmap2 pos2 impl).
+  Proof.
+    intros. destruct impl as [ [args rets] body ]. ignore_positions.
+    apply compile_stmt_length_ignores_positions.
+  Qed.
+
+  Lemma build_fun_pos_env_ignores_posmap_aux: forall posmap1 posmap2 e i1 m1 i2 m2,
+      map.fold (FlatToRiscvDef.add_compiled_function posmap1) ([], map.empty) e = (i1, m1) ->
+      map.fold (FlatToRiscvDef.add_compiled_function posmap2) ([], map.empty) e = (i2, m2) ->
+      m1 = m2 /\ List.length i1 = List.length i2.
+  Proof.
+    intros until e.
+    eapply map.fold_parametricity with (fa := (FlatToRiscvDef.add_compiled_function posmap1))
+                                       (fb := (FlatToRiscvDef.add_compiled_function posmap2));
+      intros.
+    - destruct a as [insts1 map1]. destruct b as [insts2 map2].
+      unfold FlatToRiscvDef.add_compiled_function in *.
+      inversion H0. inversion H1. subst. clear H0 H1.
+      specialize H with (1 := eq_refl) (2 := eq_refl). destruct H.
+      rewrite ?H0. subst.
+      split. 1: reflexivity.
+      ignore_positions.
+      apply compile_function_length_ignores_positions.
+    - inversion H. inversion H0. subst. auto.
+  Qed.
+
+  Lemma build_fun_pos_env_ignores_posmap: forall posmap1 posmap2 e,
+      snd (map.fold (FlatToRiscvDef.add_compiled_function posmap1) ([], map.empty) e) =
+      snd (map.fold (FlatToRiscvDef.add_compiled_function posmap2) ([], map.empty) e).
+  Proof.
+    intros.
+    destr (map.fold (FlatToRiscvDef.add_compiled_function posmap1) ([], map.empty) e).
+    destr (map.fold (FlatToRiscvDef.add_compiled_function posmap2) ([], map.empty) e).
+    simpl.
+    edestruct build_fun_pos_env_ignores_posmap_aux.
+    - exact E.
+    - exact E0.
+    - assumption.
+  Qed.
+
+  (* This lemma should relate two map.folds which fold two different f over the same env e:
+     1) FlatToRiscvDef.compile_funs, which folds FlatToRiscvDef.add_compiled_function.
+        Note that this one is called twice: First in build_fun_pos_env, and then in
+        compile_funs, and we rely on the order being the same both times.
+     2) functions, which folds sep
+     Note that 1) is not commutative (the iteration order determines in which order code
+     is layed out in memory), while 2) should be commutative because the "function"
+     separation logic predicate it seps onto the separation logic formula is the same
+     if we pass it the same function position map. *)
+  Lemma functions_to_program: forall functions_start e instrs pos_map stack_size,
+      riscvPhase e = Some (instrs, pos_map, stack_size) ->
+      iff1 (program iset functions_start instrs)
+           (FlatToRiscvCommon.functions functions_start (FlatToRiscvDef.build_fun_pos_env e) e).
+  Proof.
+    (* PARAMRECORDS *)
+    assert (map.ok FlatImp.env). { unfold FlatImp.env. simpl. typeclasses eauto. }
+    assert (map.ok mem) as Ok by exact mem_ok.
+
+    unfold riscvPhase.
+    intros.
+    simp.
+    unfold FlatToRiscvDef.compile_funs, functions in *.
+    remember (FlatToRiscvDef.build_fun_pos_env e) as positions.
+    (* choose your IH carefully! *)
+    lazymatch goal with
+    | |- ?G => enough ((forall f, map.get r f <> None <-> map.get e f <> None) /\
+                       ((forall f pos, map.get r f = Some pos -> map.get positions f = Some pos) -> G))
+    end.
+    1: {
+      destruct H0. apply H1; clear H1.
+      intros. rewrite <- H1. f_equal.
+      subst.
+      apply (f_equal snd) in E0. simpl in E0. rewrite <- E0.
+      transitivity (snd (map.fold (FlatToRiscvDef.add_compiled_function map.empty) ([], map.empty) e)).
+      - unfold FlatToRiscvDef.build_fun_pos_env, snd. reflexivity.
+      - apply build_fun_pos_env_ignores_posmap.
+    }
+    revert E0.
+    revert instrs r. clear E stack_size.
+    eapply (map.fold_spec (R:=(list Instruction * _))) with (m:=e); repeat (cbn || simp || intros).
+    { rewrite map.fold_empty. intuition try reflexivity.
+      - eapply H0. eapply map.get_empty.
+      - eapply H0. eapply map.get_empty.
+    }
+    rewrite map.fold_put; trivial.
+    2: { intros.
+      eapply functional_extensionality_dep; intros x.
+      eapply PropExtensionality.propositional_extensionality; revert x.
+      match goal with |- forall x, ?P x <-> ?Q x => change (iff1 P Q) end.
+      cancel. }
+    case r as (instrs'&r').
+    specialize H1 with (1 := eq_refl).
+    unfold FlatToRiscvDef.add_compiled_function in E0.
+    injection E0; clear E0; intros. subst.
+    unfold program in *.
+    wseplog_pre.
+    destruct H1.
+    split. {
+      intros. rewrite ?map.get_put_dec.
+      destr (k =? f)%string. 2: eauto. intuition discriminate.
+    }
+    intros.
+    rewrite H2. 2: {
+      intros.
+      eapply H3.
+      rewrite map.get_put_dec.
+      destr (k =? f)%string. 2: assumption.
+      subst. exfalso.
+      specialize (H1 f). unfold not in H1. rewrite H0 in H1. rewrite H4 in H1.
+      intuition congruence.
+    }
+    cancel.
+    unfold function.
+    specialize (H3 k).
+    rewrite map.get_put_same in H3.
+    specialize H3 with (1 := eq_refl).
+    simpl in *. rewrite H3.
+    cancel.
+    unfold program.
+    cancel_seps_at_indices 0%nat 0%nat. 2: reflexivity.
+    f_equal.
+    f_equal.
+    solve_word_eq word_ok.
+  Qed.
+
+  Open Scope ilist_scope.
+
+  Definition machine_ok(p_functions: word)(f_entry_rel_pos: Z)(stack_start stack_pastend: word)
+             (finstrs: list Instruction)
+             (p_call pc: word)(mH: mem)(Rdata Rexec: mem -> Prop)(mach: MetricRiscvMachine): Prop :=
+      let CallInst := Jal RegisterNames.ra
+                          (f_entry_rel_pos + word.signed (word.sub p_functions p_call)) : Instruction in
+      (program iset p_functions finstrs *
+       program iset p_call [CallInst] *
+       mem_available stack_start stack_pastend *
+       Rdata * Rexec * eq mH
+      )%sep mach.(getMem) /\
+      subset (footpr (program iset p_functions finstrs *
+                      program iset p_call [CallInst] *
+                      Rexec)%sep)
+             (of_list (getXAddrs mach)) /\
+      word.unsigned (mach.(getPc)) mod 4 = 0 /\
+      mach.(getPc) = pc /\
+      mach.(getNextPc) = word.add mach.(getPc) (word.of_Z 4) /\
+      regs_initialized mach.(getRegs) /\
+      map.get mach.(getRegs) RegisterNames.sp = Some stack_pastend /\
+      (* configured by PrimitivesParams, can contain invariants needed for external calls *)
+      valid_machine mach.
+
+  (* handwritten "related" (rather than composition of all phases), and restricted to
+     argument-less function calls (compiling general snippets need more context for
+     FlatToRiscv, namely function positions) and thus simpler *)
+  Definition manual_related(f1: Semantics.env * Syntax.cmd.cmd)(s1: SrcState)
+                           (f2: GhostConsts)(mach: MetricRiscvMachine): Prop :=
+    let '(functions, c) := f1 in
+    let '(functions', c', done, t, mH, lH, mcH) := s1 in
+    functions' = functions /\
+    c' = c /\
+    mach.(getLog) = t /\
+    (done = false -> lH = map.empty) /\
+    exists f_entry_name f_entry_rel_pos (finstrs: list Instruction) stack_start stack_words_needed,
+      c = Syntax.cmd.call [] f_entry_name [] /\
+      ExprImp.valid_funs functions /\
+      composed_compile functions = Some (finstrs, f2.(e_pos), stack_words_needed) /\
+      map.get f2.(e_pos) f_entry_name = Some f_entry_rel_pos /\
+      machine_ok f2.(program_base) f_entry_rel_pos
+                 stack_start f2.(p_sp) finstrs
+                 f2.(p_insts) (if done then (word.add f2.(p_insts) (word.of_Z 4)) else f2.(p_insts))
+                 mH f2.(FlatToRisc... ? dframe) f2.(xframe) mach /\
+      f2.(rem_stackwords) = word.unsigned (word.sub f2.(p_sp) stack_start) /\
+      f2.(rem_framewords) = 0 /\
+      stack_words_needed <= f2.(rem_stackwords) / bytes_per_word /\
+      f2.(insts) = [[Jal RegisterNames.ra
+                         (f_entry_rel_pos + word.signed (word.sub f2.(program_base) f2.(p_insts)))]].
+
+manual_related new?
+
+  Ltac sim'_destructible T :=
+    lazymatch T with
+    | prod _ _ => idtac
+    | SrcState => idtac
+    | FlatState _ => idtac
+    | GhostConsts => idtac
+    end.
+
+  Lemma rename_functions_related: forall e1 e2,
+    rename_functions e1 = Some e2 ->
+    RegRename.envs_related e1 e2.
+  Proof.
+    intros.
+    unfold envs_related.
+    intros f [ [argnames resnames] body1 ] G.
+    unfold rename_functions in *.
+    eapply map.map_all_values_fw.
+    5: exact G. 4: eassumption.
+    - eapply String.eqb_spec.
+    - typeclasses eauto.
+    - typeclasses eauto.
+  Qed.
+
+  Create HintDb simpl_related.
+  Hint Resolve rename_functions_related : simpl_related.
+
+
+  (* Some compilation phases establish some kind of "validFrame" for the target language,
+     eg spilling guarantees that all register names are <32 *, and these "validFrame"
+     conditions are then needed by the next phase's "related".
+     (making "validFrame" a distinct concept might be overkill, and not work so well for
+     risc-v because it would need the high-level memory as well to split the memory).
+     Filling in the intermediate existentials created by compose_related and showing that
+     the compilation of phase i respects the "validFrame" conditions of phase i+1 is the
+     purpose of this proof. *)
+
+  (* where to go from "compile hl = ll" to "envs_related hl ll"?
+     ideally in each phase simulation, rather than after the composition *)
+
+  Lemma sim': simulation srcExec runsTo manual_related.
+  Proof.
+    eapply specialize_simulation_frames. 3: eapply sim.
+    - unfold related, compose_related.
+      unfold flattening_related, renaming_related, spilling_related, flat_related_to_riscv.
+      unfold manual_related, machine_ok, goodMachine.
+      unfold composed_compile, composePhases.
+      unfold flattenPhase, renamePhase, spillingPhase, riscvPhase.
+
+Ltac step := match goal with
+             | x: ?T |- _ => sim'_destructible T; destruct x
+             | |- forall _, _ => intros
+             | |- _ => progress (cbn in *; simp)
+             | |- exists x: ?T, _ =>
+               let y := fresh x in unshelve epose (_: T) as y;
+               [ repeat lazymatch goal with
+                        | |- ?T => sim'_destructible T; econstructor
+                        end;
+                 shelve
+               | exists y; subst y ]
+             | |- _ /\ _ => split
+           (*| |- ?G => assert_fails (has_evar G); reflexivity*)
+             | |- ?G => reflexivity
+             | |- _ => eauto 3 with simpl_related
+             end.
+
+      repeat step.
+
+
+      {
+
+Search r3.
+
+(* problem with GhostConsts: contains e_impl, which is a concept from FlatImp, can't easily
+   be derived by looking at RiscvMachine state (would need to decompile) *)
+
+  E2 : FlatToRiscvDef.compile_funs (FlatToRiscvDef.build_fun_pos_env (spill_functions r3))
+         (spill_functions r3) = (finstrs, r4)
+
+spill_functions r3 = e_impl   ?
+
+
+Set Ltac Profiling.
+
+Set Nested Lemmas.
+
+
+E0: rename_functions r1 = Some r3
+
+
+      Search r1.
+
+Show Ltac Profile.
+
+total time:     32.688s
+
+ tactic                                   local  total   calls       max
+────────────────────────────────────────┴──────┴──────┴───────┴─────────┘
+─step ----------------------------------  99.8% 100.0%     326   11.103s
+─simp ----------------------------------   0.0%  96.8%     228   11.085s
+─simp_step -----------------------------   0.1%  96.7%     153    0.577s
+─destruct_unique_match -----------------  71.2%  71.2%    2271    0.383s
+─destruct e eqn:N ----------------------  37.6%  37.6%     620    0.057s
+─unique_inversion ----------------------  25.4%  25.4%    4647    0.253s
+─protect_equalities --------------------   8.1%  16.8%    4333    0.015s
+─congruence ----------------------------  13.2%  13.2%    1508    0.018s
+─change_no_check (protected (a = b)) in    8.7%   8.7%   19512    0.011s
+─elimtype ------------------------------   7.3%   7.3%    3021    0.014s
+─discriminate --------------------------   5.7%   5.7%    1513    0.015s
+─destruct e ----------------------------   4.8%   4.8%     137    0.036s
+
+ tactic                                   local  total   calls       max
+────────────────────────────────────────┴──────┴──────┴───────┴─────────┘
+─step ----------------------------------  99.8% 100.0%     326   11.103s
+└simp ----------------------------------   0.0%  96.8%     228   11.085s
+└simp_step -----------------------------   0.1%  96.7%     153    0.577s
+ ├─destruct_unique_match ---------------  71.2%  71.2%    2271    0.383s
+ │ ├─destruct e eqn:N ------------------  37.6%  37.6%     620    0.057s
+ │ ├─congruence ------------------------  13.2%  13.2%    1508    0.018s
+ │ ├─elimtype --------------------------   7.3%   7.3%    3021    0.014s
+ │ ├─discriminate ----------------------   5.7%   5.7%    1513    0.015s
+ │ └─destruct e ------------------------   4.8%   4.8%     137    0.036s
+ └─unique_inversion --------------------  25.4%  25.4%    4647    0.253s
+  └protect_equalities ------------------   8.1%  16.8%    4333    0.015s
+  └change_no_check (protected (a = b)) i   8.7%   8.7%   19512    0.011s
+
+      Search r.
+
+      step.
+      step.
+      step.
+      step.
+      step.
+      step.
+      step.
+      step.
+      step.
+      step.
+      step.
+      step.
+
+
+step.
+      step.
+      step.
+      step.
+      step.
+      step.
+      step.
+
+      repeat match goal with
+             | x: ?T |- _ => sim'_destructible T; destruct x
+             | |- _ => progress (cbn in *; simp)
+             | |- exists x: ?T, _ =>
+               let y := fresh x in unshelve epose (_: T) as y;
+               [ repeat lazymatch goal with
+                        | |- ?T => sim'_destructible T; econstructor
+                        end;
+                 shelve | ]
+             end.
+      match goal with
+      | |- exists x: ?T, _ =>
+        sim'_destructible T;
+        let y := fresh x in unshelve epose (_: T) as y
+      end.
+      { econstructor; shelve. }
+      exists f2. subst f2.
+      cbn.
+      match goal with
+      | |- exists x: ?T, _ =>
+        let y := fresh x in unshelve epose (_: T) as y
+      end.
+      { repeat lazymatch goal with
+               | |- ?T => sim'_destructible T; econstructor
+               end;
+          shelve. }
+      exists s0.
+      subst s0.
+      cbn.
+
+ econstructor.
+
+      match goal with
+      | |- exists x: ?T, _ =>
+        sim'_destructible T;
+        let y := fresh x in evar (y: T)
+      end.
+      exists f2.
+      destruct f2 eqn: E.
+
+      cbn.
+
+      destruct f2.
+      ma
+      intros (e & c).
+      intros ((? & ?) & ?).
+
+
+ (e' & c
+      intros. simp.
+
+
+case TODO.
+    - case TODO.
+  Qed.
+
+  Definition compile(ml: MemoryLayout)(p: source_env): option (list Instruction * funname_env Z) :=
+    match composed_compile p with
+    | Some (insts, positions, stack_words_needed) =>
+      let num_stackwords := word.unsigned (word.sub ml.(stack_pastend) ml.(stack_start)) / bytes_per_word in
+      if Z.ltb num_stackwords stack_words_needed then None (* not enough stack *) else Some (insts, positions)
+    | None => None
+    end.
+
+  (* This lemma translates "sim", which depends on the large definition "related", into something
+     more understandable and usable. *)
+  Lemma compiler_correct: forall
+      (ml: MemoryLayout)
+      (mlOk: MemoryLayoutOk ml)
+      (f_entry_name : string) (fbody: Syntax.cmd.cmd) (f_entry_rel_pos: Z)
+      (p_call p_functions: word)
+      (Rdata Rexec : mem -> Prop)
+      (functions: source_env)
+      (instrs: list Instruction)
+      (pos_map: funname_env Z)
+      (mH: mem) (mc: MetricLog)
+      (postH: Semantics.trace -> Semantics.mem -> Prop)
+      (initial: MetricRiscvMachine),
+      ExprImp.valid_funs functions ->
+      compile ml functions = Some (instrs, pos_map) ->
+      map.get functions f_entry_name = Some (nil, nil, fbody) ->
+      map.get pos_map f_entry_name = Some f_entry_rel_pos ->
+      Semantics.exec functions fbody initial.(getLog) mH map.empty mc (fun t' m' l' mc' => postH t' m') ->
+      machine_ok p_functions f_entry_rel_pos ml.(stack_start) ml.(stack_pastend) instrs
+                 p_call p_call mH Rdata Rexec initial ->
+      runsTo initial (fun final => exists mH',
+          postH final.(getLog) mH' /\
+          machine_ok p_functions f_entry_rel_pos ml.(stack_start) ml.(stack_pastend) instrs
+                     p_call (word.add p_call (word.of_Z 4)) mH' Rdata Rexec final).
+  Proof.
+    intros. unfold compile in *. simp. eapply Z.ltb_ge in E0.
+    eapply runsTo_weaken.
+    - pose proof sim' as P. eapply simulation_alt in P.
+      unfold simulation_without_weakening, SrcState, srcExec in P.
+      let x := open_constr:((_, _, false, _, _, _, _):
+        Semantics.env * Syntax.cmd.cmd * bool * Semantics.trace * Semantics.mem * Semantics.locals * MetricLog)
+      in specialize P with (s1 := x).
+      let x := open_constr:((_, _): Semantics.env * Syntax.cmd.cmd)
+      in specialize P with (f1 := x).
+      specialize P with (P1 := fun '(e', c', done', t', m', l', mc') =>
+                 e' = functions /\ c' = Syntax.cmd.call [] f_entry_name [] /\ done' = true /\ postH t' m').
+      let x := open_constr:({| p_sp := _ |}) in specialize (P x initial).
+      simpl in P.
+      eapply P; clear P.
+      + repeat match goal with
+               | |- _ /\ _ => split
+               | |- exists _, _ => eexists
+               | |- _ => reflexivity
+               | |- _ => eassumption
+               end.
+      + split; [reflexivity|].
+        eapply Semantics.exec.call; try eassumption || reflexivity.
+        cbv beta. intros.
+        repeat match goal with
+               | |- _ /\ _ => split
+               | |- exists _, _ => eexists
+               | |- _ => reflexivity
+               | |- _ => eassumption
+               end.
+    - cbv beta. intros. simp. eexists. split; [eassumption|].
+      match goal with
+      | H: ?P |- ?Q => let hP := head_of_app P in let hQ := head_of_app Q in constr_eq hP hQ;
+                       replace Q with P; [exact H|f_equal]
+      end.
+      + blia.
+      + rename H0p0p3p5 into A. clear -A h.
+        (* TODO how to automate this one? *)
+        apply (f_equal word.of_Z) in A. rewrite ?@word.of_Z_unsigned in A. 2,3: typeclasses eauto.
+        apply (f_equal (word.sub (stack_pastend ml))) in A.
+        ring_simplify in A.
+        symmetry in A.
+        exact A.
+      + congruence.
+    Unshelve. all: try exact map.empty.
+  Qed.
+
+  (* Old proof: *)
+  Goal forall
+      (ml: MemoryLayout)
+      (mlOk: MemoryLayoutOk ml)
+      (f_entry_name : string) (fbody: Syntax.cmd.cmd) (f_entry_rel_pos: Z)
+      (p_call p_functions: word)
+      (Rdata Rexec : mem -> Prop)
+      (functions: source_env)
+      (instrs: list Instruction)
+      (pos_map: funname_env Z)
+      (mH: mem) (mc: MetricLog)
+      (postH: Semantics.trace -> Semantics.mem -> Prop)
+      (initial: MetricRiscvMachine),
+      ExprImp.valid_funs functions ->
+      compile ml functions = Some (instrs, pos_map) ->
+      map.get functions f_entry_name = Some (nil, nil, fbody) ->
+      map.get pos_map f_entry_name = Some f_entry_rel_pos ->
+      Semantics.exec functions fbody initial.(getLog) mH map.empty mc (fun t' m' l' mc' => postH t' m') ->
+      machine_ok p_functions f_entry_rel_pos ml.(stack_start) ml.(stack_pastend) instrs
+                 p_call p_call mH Rdata Rexec initial ->
+      runsTo initial (fun final => exists mH',
+          postH final.(getLog) mH' /\
+          machine_ok p_functions f_entry_rel_pos ml.(stack_start) ml.(stack_pastend) instrs
+                     p_call (word.add p_call (word.of_Z 4)) mH' Rdata Rexec final).
+  Proof.
+    intros.
+    match goal with
+    | H: map.get pos_map _ = Some _ |- _ => rename H into GetPos
+    end.
+    unfold compile, composed_compile, composePhases, flattenPhase, renamePhase, spillingPhase in *. simp.
+
+    match goal with
+    | H: flatten_functions _ = _ |- _ => rename H into FlattenEq
+    end.
+    unfold flatten_functions in FlattenEq.
+    match goal with
+    | H: _ |- _ => unshelve epose proof (map.map_all_values_fw _ _ _ _ FlattenEq _ _ H)
+    end.
+    simp.
+    match goal with
+    | H: rename_functions _ = _ |- _ => rename H into RenameEq
+    end.
+    unfold rename_functions in RenameEq.
+    match goal with
+    | H: _ |- _ => unshelve epose proof (map.map_all_values_fw _ _ _ _ RenameEq _ _ H)
+    end.
+    simp.
+    match goal with
+    | H: flatten_function _ = _ |- _ => rename H into FF
+    end.
+    unfold flatten_function in FF. simp.
+
+    eapply runsTo_weaken.
+    - pose proof sim as P. eapply simulation_alt in P.
+      unfold simulation_without_weakening, SrcState, srcExec in P.
+      let x := open_constr:((_, _, _, _, _, _, _):
+        Semantics.env * Syntax.cmd.cmd * bool * Semantics.trace * Semantics.mem * Semantics.locals * MetricLog)
+      in specialize P with (s1 := x).
+      let x := open_constr:((_, _): Semantics.env * Syntax.cmd.cmd)
+      in specialize P with (f1 := x).
+      specialize P with (P1 := fun '(e', c', done', t', m', l', mc') =>
+                                 e' = functions /\ c' = fbody /\ done' = true /\ postH t' m').
+      simpl in P.
+      eapply P; clear P. 2: {
+        split; [reflexivity|]. eapply ExprImp.weaken_exec. 1: eassumption.
+        cbv beta. eauto.
+      }
+      unfold related, flattening_related, renaming_related, spilling_related, flat_related_to_riscv,
+             compose_related.
+      eexists (_, _), (_, _, _, _, _, _, _).
+      all: admit.
+      (*
+      ssplit; try reflexivity; eauto.
+      { eexists.
+        match goal with
+        | |- ?x = (?evar1, ?evar2) => transitivity (fst x, snd x)
+        end.
+        2: reflexivity.
+        match goal with
+        | |- ?x = (_, _) => destruct x; reflexivity
+        end. }
+      eexists (_, _), (_, _, _, _, _, _, _).
+      ssplit; try reflexivity; eauto.
+      { unfold envs_related.
+        intros f [ [argnames resnames] body1 ] G.
+        unfold rename_functions in *.
+        eapply map.map_all_values_fw.
+        5: exact G. 4: eassumption.
+        - eapply String.eqb_spec.
+        - typeclasses eauto.
+        - simpl. typeclasses eauto.
+      }
+      refine (ex_intro _ (_, _, _, _) _).
+      ssplit; try reflexivity.
+      { intros. ssplit; reflexivity. }
+      { unfold machine_ok in *. simp.
+        (* PARAMRECORDS *) simpl.
+        solve_word_eq word_ok. }
+      unfold goodMachine. simpl. ssplit.
+      { simpl. unfold map.extends. intros k v Emp. rewrite map.get_empty in Emp. discriminate. }
+      { simpl. unfold map.extends. intros k v Emp. rewrite map.get_empty in Emp. discriminate. }
+      { simpl. unfold machine_ok in *. simp. assumption. }
+      { unfold machine_ok in *. simp. assumption. }
+      { unfold machine_ok in *. simp. assumption. }
+      { unfold machine_ok in *. simp. simpl.
+        eapply rearrange_footpr_subset. 1: eassumption.
+        (* COQBUG https://github.com/coq/coq/issues/11649 *)
+        pose proof (mem_ok: @map.ok (@word (@W p)) Init.Byte.byte (@mem p)).
+        wwcancel.
+        eapply functions_to_program.
+        eassumption. }
+      { simpl.
+        (* COQBUG https://github.com/coq/coq/issues/11649 *)
+        pose proof (mem_ok: @map.ok (@word (@W p)) Init.Byte.byte (@mem p)).
+        unfold machine_ok in *. simp.
+        edestruct mem_available_to_exists as [ stack_trash [? ?] ]. 1: simpl; ecancel_assumption.
+        destruct (byte_list_to_word_list_array stack_trash)
+          as (stack_trash_words&Hlength_stack_trash_words&Hstack_trash_words).
+        { rewrite H4.
+          apply stack_length_divisible.
+          assumption. }
+        exists stack_trash_words.
+        split. 2: {
+          unfold word_array.
+          rewrite <- (iff1ToEq (Hstack_trash_words _)).
+          match goal with
+          | E: Z.of_nat _ = word.unsigned (word.sub _ _) |- _ => simpl in E|-*; rewrite <- E
+          end.
+          lazymatch goal with
+          | H: riscvPhase _ _ = _ |- _ => specialize functions_to_program with (1 := H) as P
+          end.
+          symmetry in P.
+          simpl in P|-*. unfold program in P.
+          seprewrite P. clear P.
+          assert (word.ok FlatImp.word) by exact word_ok.
+          rewrite <- Z_div_exact_2; cycle 1. {
+            unfold bytes_per_word. clear -h.
+            destruct width_cases as [E | E]; rewrite E; reflexivity.
+          }
+          {
+            match goal with
+            | H: ?x = ?y |- _ => rewrite H
+            end.
+            apply stack_length_divisible.
+            assumption.
+          }
+          wcancel_assumption.
+          rewrite word.of_Z_unsigned.
+          cancel_seps_at_indices O O. {
+            (* PARAMRECORDS *) simpl.
+            sepclause_eq word_ok.
+          }
+          cbn [seps]. reflexivity.
+        }
+        match goal with
+        | E: Z.of_nat _ = word.unsigned (word.sub _ _) |- _ => simpl in E|-*; rewrite <- E
+        end.
+        rewrite Z.sub_0_r. symmetry.
+        apply Hlength_stack_trash_words. }
+      { reflexivity. }
+      { unfold machine_ok in *. simp. assumption. }
+      *)
+    - intros. unfold compile_inv, related, compose_related in *.
+      match goal with
+      | H: context[machine_ok] |- _ =>
+        unfold machine_ok in H;
+        repeat match type of H with
+               | _ /\ _ => let A := fresh "HOK0" in destruct H as [A H];
+                           lazymatch type of A with
+                           | verify _ _ => idtac
+                           | _ = p_call => idtac
+                         (*| _ => clear A*)
+                           end
+               end
+      end.
+      subst.
+      repeat match goal with
+             | H: context[Semantics.exec] |- _ => clear H
+             end.
+      unfold flattening_related, renaming_related, spilling_related, flat_related_to_riscv in *.
+      unfold FlatToRiscvSimulation.related, FlattenExprSimulation.related, RegRename.related, goodMachine in *.
+      admit.
+      (*
+      simp.
+      eexists. split. 1: eassumption.
+      unfold machine_ok. ssplit; try assumption.
+      + assert (map.ok mem). { exact mem_ok. } (* PARAMRECORDS *)
+        cbv [rem_stackwords rem_framewords ghostConsts] in H2p0p1p8p0.
+        cbv [mem_available].
+        repeat rewrite ?(iff1ToEq (sep_ex1_r _ _)), ?(iff1ToEq (sep_ex1_l _ _)).
+        exists (List.flat_map (fun x => HList.tuple.to_list (LittleEndian.split (Z.to_nat bytes_per_word) (word.unsigned x))) stack_trash).
+        rewrite !(iff1ToEq (sep_emp_2 _ _ _)).
+        rewrite !(iff1ToEq (sep_assoc _ _ _)).
+        eapply (sep_emp_l _ _); split.
+        { assert (0 < bytes_per_word). { (* TODO: deduplicate *)
+            unfold bytes_per_word; simpl; destruct width_cases as [EE | EE]; rewrite EE; cbv; trivial.
+          }
+          rewrite (length_flat_map _ (Z.to_nat bytes_per_word)).
+          { rewrite Nat2Z.inj_mul, Z2Nat.id by blia. rewrite Z.sub_0_r in H2p0p1p8p0.
+            rewrite <-H2p0p1p8p0, <-Z_div_exact_2; try trivial.
+            { eapply Z.lt_gt; assumption. }
+            { eapply stack_length_divisible; trivial. } }
+          intros w.
+          rewrite HList.tuple.length_to_list; trivial. }
+        use_sep_assumption.
+        cbn [dframe xframe ghostConsts program_base ghostConsts e_pos e_impl p_insts insts].
+        progress simpl (@FlatToRiscvCommon.mem (@FlatToRiscv_params p)).
+        wwcancel.
+        cancel_seps_at_indices 0%nat 3%nat. {
+          reflexivity.
+        }
+        cancel_seps_at_indices 0%nat 2%nat. {
+          cbn [rem_stackwords rem_framewords ghostConsts p_sp].
+          replace (word.sub (stack_pastend ml) (word.of_Z (bytes_per_word *
+                      (word.unsigned (word.sub (stack_pastend ml) (stack_start ml)) / bytes_per_word))))
+            with (stack_start ml). 2: {
+            rewrite <- Z_div_exact_2; cycle 1. {
+              unfold bytes_per_word. clear -h. simpl.
+              destruct width_cases as [E | E]; rewrite E; reflexivity.
+            }
+            {
+              apply stack_length_divisible.
+              assumption.
+            }
+            rewrite word.of_Z_unsigned.
+            solve_word_eq word_ok.
+          }
+          apply iff1ToEq, cast_word_array_to_bytes.
+        }
+        unfold ptsto_instr.
+        simpl.
+        unfold ptsto_bytes, ptsto_instr, truncated_scalar, littleendian, ptsto_bytes.ptsto_bytes.
+        simpl.
+        assert (map.ok mem). { exact mem_ok. } (* PARAMRECORDS *)
+        wwcancel.
+        epose proof (functions_to_program ml _ r0 instrs) as P.
+        cbn [seps].
+        rewrite <- P; clear P.
+        * wwcancel. reflexivity.
+        * eassumption.
+      + unfold machine_ok in *. simp. simpl.
+        eapply rearrange_footpr_subset. 1: eassumption.
+        (* COQBUG https://github.com/coq/coq/issues/11649 *)
+        pose proof (mem_ok: @map.ok (@word (@W p)) Init.Byte.byte (@mem p)).
+        (* TODO remove duplication *)
+        lazymatch goal with
+        | H: riscvPhase _ _ = _ |- _ => specialize functions_to_program with (1 := H) as P
+        end.
+        symmetry in P.
+        rewrite P. clear P.
+        cbn [dframe xframe ghostConsts program_base ghostConsts e_pos e_impl p_insts insts program].
+        simpl.
+        unfold ptsto_bytes, ptsto_instr, truncated_scalar, littleendian, ptsto_bytes.ptsto_bytes.
+        simpl.
+        wwcancel.
+      + destr_RiscvMachine final. subst. solve_divisibleBy4.
+      *)
+    Unshelve.
+    all: try exact (bedrock2.MetricLogging.mkMetricLog 0 0 0 0).
+    all: try (simpl; typeclasses eauto).
+    all: try exact EmptyString.
+    all: try exact nil.
+    all: try exact map.empty.
+    all: try exact mem_ok.
+  Abort.
+
+  Definition instrencode(p: list Instruction): list byte :=
+    List.flat_map (fun inst => HList.tuple.to_list (LittleEndian.split 4 (encode inst))) p.
+
+End Pipeline1.
