compiler/src/compiler/UpperPipeline.v
@@ -1,0 +1,308 @@
+Require Export Coq.Lists.List.
+Require Import Coq.ZArith.ZArith.
+Export ListNotations.
+Require Import coqutil.Decidable.
+Require Import coqutil.Z.Lia.
+Require Import coqutil.Tactics.Simp.
+Require Import bedrock2.MetricLogging.
+Require Import compiler.ExprImp.
+Require Import compiler.FlattenExprDef.
+Require Import compiler.FlattenExpr.
+Require Import compiler.FlatImp.
+Require Import compiler.NameGen.
+Require Import compiler.StringNameGen.
+Require Import compiler.util.Common.
+Require Import compiler.SeparationLogic.
+Require Import compiler.Spilling.
+Require Import compiler.RegRename.
+
+Section WithWordAndMem.
+  Context {width: Z} {word: Interface.word width} {mem : map.map word byte}.
+
+  (* TODO put into common file *)
+  Definition trace: Type := list (mem * string * list word * (mem * list word)).
+  Definition ExtSpec: Type := trace -> mem -> string -> list word -> (mem -> list word -> Prop) -> Prop.
+
+  Record Lang: Type := {
+    Var: Type;
+    Cmd: Type;
+    Locals : map.map Var word;
+    Env : map.map string (list Var * list Var * Cmd);
+    Exec: Env -> Cmd -> trace -> mem -> Locals -> MetricLog ->
+          (trace -> mem -> Locals -> MetricLog -> Prop) -> Prop
+  }.
+
+  Definition relation(L1 L2: Lang): Type := bool ->
+    L1.(Env) -> L1.(Cmd) -> trace -> mem -> L1.(Locals) -> MetricLog ->
+    L2.(Env) -> L2.(Cmd) -> trace -> mem -> L2.(Locals) -> MetricLog -> Prop.
+
+  Definition simulation{L1 L2: Lang}(R: relation L1 L2) :=
+    forall (e1: L1.(Env)) (e2: L2.(Env)) (c1: L1.(Cmd)) (c2: L2.(Cmd))
+           (P1: trace -> mem -> L1.(Locals) -> MetricLog -> Prop)
+           (P2: trace -> mem -> L2.(Locals) -> MetricLog -> Prop),
+      (forall t1 m1 l1 mc1 t2 m2 l2 mc2, R true e1 c1 t1 m1 l1 mc1 e2 c2 t2 m2 l2 mc2 ->
+                                         P1 t1 m1 l1 mc1 -> P2 t2 m2 l2 mc2) ->
+      (forall t1 m1 l1 mc1 t2 m2 l2 mc2, R false e1 c1 t1 m1 l1 mc1 e2 c2 t2 m2 l2 mc2 ->
+                                         L1.(Exec) e1 c1 t1 m1 l1 mc1 P1 ->
+                                         L2.(Exec) e2 c2 t2 m2 l2 mc2 P2).
+
+  Definition compose_related{L1 L2 L3: Lang}(R12: relation L1 L2)(R23: relation L2 L3): relation L1 L3 :=
+    fun done e1 c1 t1 m1 l1 mc1 e3 c3 t3 m3 l3 mc3 =>
+      exists e2 c2 t2 m2 l2 mc2, R12 done e1 c1 t1 m1 l1 mc1 e2 c2 t2 m2 l2 mc2 /\
+                                 R23 done e2 c2 t2 m2 l2 mc2 e3 c3 t3 m3 l3 mc3.
+
+  Lemma compose_simulation{L1 L2 L3: Lang}{R12: relation L1 L2}{R23: relation L2 L3}
+        (S12: simulation R12)(S23: simulation R23): simulation (compose_related R12 R23).
+  Proof.
+    unfold simulation, compose_related in *.
+    intros e1 e3 c1 c3 P1 P3 W t1 m1 l1 mc1 t3 m3 l3 mc3 R13 Ex1.
+    simp.
+    eapply S23. 2: eassumption. 2: {
+      eapply S12 with (P2 := (fun t2' m2' l2' mc2' => exists t1' m1' l1' mc1',
+                                  R12 true e1 c1 t1' m1' l1' mc1' e2 c2 t2' m2' l2' mc2' /\
+                                  P1 t1' m1' l1' mc1')).
+      3: eassumption. 2: eassumption. clear. eauto 10.
+    }
+    cbv beta. clear -W. intros. simp. eauto 10.
+  Qed.
+
+  Section WithMoreParams.
+    Context {Zlocals: map.map Z word}
+            {string_keyed_map: forall T: Type, map.map string T} (* abstract T for better reusability *)
+            (ext_spec: ExtSpec)
+            (width_cases : width = 32 \/ width = 64)
+            {word_ok : word.ok word}
+            {mem_ok: map.ok mem}
+            {string_keyed_map_ok: forall T, map.ok (string_keyed_map T)}
+            {Zlocals_ok: map.ok Zlocals}.
+
+    Instance W: Words := {| Utility.width_cases := width_cases |}.
+
+    Instance FlattenExpr_parameters: FlattenExpr.parameters := {
+      FlattenExpr.W := _;
+      FlattenExpr.locals := _;
+      FlattenExpr.mem := mem;
+      FlattenExpr.ext_spec := ext_spec;
+      FlattenExpr.NGstate := N;
+    }.
+
+    Context {ext_spec_ok : Semantics.ext_spec.ok (FlattenExpr.mk_Semantics_params FlattenExpr_parameters)}.
+
+    Definition SrcLang := {|
+      Var := string;
+      Cmd := Syntax.cmd;
+      Env := string_keyed_map (list string * list string * Syntax.cmd);
+      Exec := Semantics.exec
+    |}.
+
+    Definition FlatLangStr := {|
+      Var := string;
+      Cmd := FlatImp.stmt string;
+      Env := string_keyed_map (list string * list string * FlatImp.stmt string);
+      Exec := FlatImp.exec
+    |}.
+
+    Instance FlatImp_params: FlatImp.parameters Z := {|
+      FlatImp.varname_eqb := Z.eqb;
+      FlatImp.ext_spec := ext_spec;
+    |}.
+
+    Definition FlatLangZ := {|
+      Var := Z;
+      Cmd := FlatImp.stmt Z;
+      Locals := Zlocals;
+      Env := string_keyed_map (list Z * list Z * FlatImp.stmt Z);
+      Exec := FlatImp.exec
+    |}.
+
+    Instance mk_FlatImp_string_ext_spec_ok:
+      FlatImp.ext_spec.ok string (FlattenExpr.mk_FlatImp_params FlattenExpr_parameters).
+    Proof.
+      destruct ext_spec_ok.
+      constructor.
+      all: intros; eauto.
+      eapply intersect; eassumption.
+    Qed.
+
+    Instance mk_FlatImp_Z_ext_spec_ok:
+      FlatImp.ext_spec.ok Z FlatImp_params.
+    Proof.
+      destruct ext_spec_ok.
+      constructor.
+      all: intros; eauto.
+      eapply intersect; eassumption.
+    Qed.
+
+    Definition flattenPhase(prog: SrcLang.(Env)): option FlatLangStr.(Env) :=
+      flatten_functions prog.
+    Definition renamePhase(prog: FlatLangStr.(Env)): option FlatLangZ.(Env) :=
+      rename_functions prog.
+    Definition spillingPhase(prog: FlatLangZ.(Env)): option FlatLangZ.(Env) :=
+      Some (spill_functions prog).
+
+    Definition composePhases{A B C: Type}(phase1: A -> option B)(phase2: B -> option C)(a: A) :=
+      match phase1 a with
+      | Some b => phase2 b
+      | None => None
+      end.
+
+    Definition composedCompileEnv: SrcLang.(Env) -> option FlatLangZ.(Env) :=
+      (composePhases flattenPhase
+      (composePhases renamePhase
+                     spillingPhase)).
+
+    Definition flattening_related: relation SrcLang FlatLangStr :=
+      fun done e1 c1 t1 m1 l1 mc1 e2 c2 t2 m2 l2 mc2 =>
+        ExprImp2FlatImp c1 = c2 /\
+        flatten_functions e1 = Some e2 /\
+        t1 = t2 /\
+        m1 = m2 /\
+        (done = false -> l1 = map.empty /\ l2 = map.empty /\ mc1 = mc2).
+
+    Lemma flattening_sim: simulation flattening_related.
+    Proof.
+      unfold simulation, flattening_related, ExprImp2FlatImp. intros.
+      simp. specialize (H0p2 eq_refl). simp.
+      eapply FlatImp.exec.weaken.
+      - eapply @flattenStmt_correct_aux with (eH := e1).
+        + econstructor; try typeclasses eauto.
+        + eassumption.
+        + eassumption.
+        + reflexivity.
+        + match goal with
+          | |- ?p = _ => rewrite (surjective_pairing p)
+          end.
+          reflexivity.
+        + intros x k A. rewrite map.get_empty in A. discriminate.
+        + unfold map.undef_on, map.agree_on. intros. reflexivity.
+        + eapply freshNameGenState_disjoint.
+      - simpl. intros. simp. eapply H. 2: eassumption. simpl. intuition (discriminate || eauto).
+    Qed.
+
+    Definition renaming_related: relation FlatLangStr FlatLangZ :=
+      fun done e1 c1 t1 m1 l1 mc1 e2 c2 t2 m2 l2 mc2 =>
+      RegRename.envs_related e1 e2 /\
+      (exists r' av', RegRename.rename map.empty c1 lowest_available_impvar = Some (r', c2, av')) /\
+      t1 = t2 /\
+      m1 = m2 /\
+      (done = false -> l1 = map.empty /\ l2 = map.empty /\ mc1 = mc2).
+
+    Lemma renaming_sim: simulation renaming_related.
+    Proof.
+      unfold simulation, renaming_related. intros.
+      simp. specialize (H0p3 eq_refl). simp.
+      pose proof H0p1 as A.
+      apply rename_props in A;
+        [|eapply map.empty_injective|eapply dom_bound_empty].
+      simp.
+      eapply FlatImp.exec.weaken.
+      - eapply rename_correct with (ext_spec0 := ext_spec).
+        1: eassumption.
+        1: eassumption.
+        3: {
+          eapply Ap2. eapply TestLemmas.extends_refl.
+        }
+        1: eassumption.
+        1: eassumption.
+        unfold states_compat. intros *. intro B.
+        erewrite map.get_empty in B. discriminate.
+      - simpl. intros. simp.
+        eapply H. 2: eassumption. simpl. clear H. intuition (discriminate || eauto).
+    Qed.
+
+    Axiom TODO: False.
+
+    Definition spilling_related: relation FlatLangZ FlatLangZ :=
+      fun done e1 c1 t1 m1 l1 mc1 e2 c2 t2 m2 l2 mc2 =>
+      c2 = spill_stmt c1 /\
+      exists maxvar (fpval: word),
+        Spilling.envs_related e1 e2 /\
+        Spilling.valid_vars_src maxvar c1 /\
+        Spilling.related ext_spec maxvar (emp True) fpval t1 m1 l1 t2 m2 l2.
+
+    Lemma spilling_sim: simulation spilling_related.
+    Proof.
+      unfold simulation, spilling_related.
+      intros. simp.
+      eapply FlatImp.exec.weaken.
+      - eapply spilling_correct with (ext_spec0 := ext_spec); eassumption.
+      - cbv beta. intros. simp. eapply H. 2: eassumption. simpl.
+        eauto 10.
+    Qed.
+
+    Definition upper_related: relation SrcLang FlatLangZ :=
+      (compose_related flattening_related
+      (compose_related renaming_related
+                       spilling_related)).
+
+    Lemma sim: simulation upper_related.
+    Proof.
+      exact (compose_simulation flattening_sim
+            (compose_simulation renaming_sim
+                                spilling_sim)).
+    Qed.
+
+    (* Note: spilling uses stackalloc to store spilled vars in the memory, so there are some points
+       in execution where the low-level memory differs from the high-level memory, but before and
+       after calling the top-level function the memories are equal, so we can simplify the correctness
+       theorem to this case *)
+
+    Lemma upper_compiler_correct: forall
+        (f_entry_name : string) (fbodyH: Syntax.cmd.cmd)
+        (functionsH: SrcLang.(Env)) (functionsL: FlatLangZ.(Env))
+        t (m: mem) (mc: MetricLog)
+        (post: Semantics.trace -> Semantics.mem -> Prop),
+        ExprImp.valid_funs functionsH ->
+        composedCompileEnv functionsH = Some functionsL ->
+        map.get functionsH f_entry_name = Some (nil, nil, fbodyH) ->
+        Semantics.exec functionsH fbodyH t m map.empty mc (fun t' m' l' mc' => post t' m') ->
+        exists fbodyL, map.get functionsL f_entry_name = Some (nil, nil, fbodyL) /\
+                       FlatImp.exec functionsL fbodyL t m map.empty mc (fun t' m' l' mc' => post t' m').
+    Proof.
+      intros.
+      unfold composedCompileEnv, composePhases in *. simp.
+      rename r into functionsF, r0 into functionsR.
+
+      pose proof E as GF.
+      unfold flattenPhase, flatten_functions in GF.
+      eapply map.map_all_values_fw in GF. 5: eassumption. 2-4: typeclasses eauto.
+      simp. unfold flatten_function in GFp0.
+      (* simp would also unfold freshNameGenState *)
+      apply Option.eq_of_eq_Some in GFp0. destruct v2 as ((? & ?) & ?).
+      eapply pair_equal_spec in GFp0. destruct GFp0 as (GFp0 & ?).
+      eapply pair_equal_spec in GFp0. destruct GFp0 as (GFp0 & ?).
+      subst.
+
+      pose proof E0 as GR.
+      unfold renamePhase, rename_functions in GR.
+      eapply map.map_all_values_fw in GR. 5: eassumption. 2-4: typeclasses eauto.
+      simp. unfold rename_fun, rename_binds in GRp0. simp.
+
+      pose proof H0 as GL.
+      unfold spillingPhase in GL. apply Option.eq_of_eq_Some in GL.
+      unfold spill_functions in GL.
+      eapply map.map_values_fw in GL. 5: eassumption. 2-4: typeclasses eauto.
+      simp. unfold spill_fun in GLp1.
+
+      eexists. split. 1: exact GLp1.
+
+      pose proof sim as Sim. unfold simulation, upper_related, Exec, SrcLang, FlatLangZ in Sim.
+      cbn in Sim. eapply Sim; clear Sim. 3: eassumption.
+
+      2: { (* upper_related holds initially: *)
+        unfold compose_related, flattening_related, renaming_related, spilling_related. cbn.
+        do 6 eexists. ssplit. all: eauto 3.
+        do 6 eexists. ssplit. all: eauto 3.
+        { unfold envs_related. intros.
+          eapply map.map_all_values_fw. 5: eassumption. 4: eassumption. all: typeclasses eauto. }
+        { unfold spill_fbody. (* oops *)
+
+    Abort.
+
+    (* Note: Spilling.related has an "exists stackwords", because after spilling, all commands are
+       always wrapped inside a stackalloc block, but if we make the command just an argument-less
+       function call, we can set stackwords to the empty list and simplify "upper_related" *)
+
+
+  End WithMoreParams.
+End WithWordAndMem.
